work on converting between 2d- and 1d- arrays

Example/Verif_arr2d.v
@@ -34,6 +34,99 @@ Definition main_spec :=
 
 Definition Gprog := [ith_spec; main_spec].
 
+Require Import VST.msl.iter_sepcon.
+
+Ltac list_solve_preprocess ::=
+  fold_Vbyte; autounfold with list_solve_unfold in *; autorewrite with
+   list_solve_rewrite in *; repeat match goal with
+                                   | |- _ /\ _ => split
+                                   end; intros.
+
+Fixpoint array_pointers_nat t p n :=
+  match n with
+  | O => []
+  | S n' => p :: (array_pointers_nat t (offset_val (sizeof t) p) n')
+  end.
+
+Definition array_pointers t p n :=
+  array_pointers_nat t p (Z.to_nat n).
+
+Lemma array_pointers_unfold t p n :
+  0 < n ->
+  array_pointers t p n = p :: (array_pointers t (offset_val (sizeof t) p) (n-1)).
+Admitted.
+
+Lemma data_at_array_iter_sepcon : forall sh t n al p,
+  0 <= n ->
+  complete_legal_cosu_type t = true ->
+  data_at sh (tarray t n) al p
+    = iter_sepcon (fun (vp : reptype t * val) => let (v, p) := vp in data_at sh t v p)
+          (combine al (array_pointers t p n)).
+Proof.
+  intros.
+  change (reptype (tarray t n)) with (list (reptype t)) in al.
+  apply pred_ext.
+  - generalize dependent n; generalize dependent p; induction al; intros.
+    + entailer!. rewrite Zlength_nil.
+      sep_apply data_at_zero_array_inv.
+      auto.
+    + assert_PROP (Zlength (a :: al) = n). { entailer!. }
+      assert_PROP (field_address0 (tarray t n) [ArraySubsc 1] p
+          = offset_val (sizeof t) p).
+      {
+        entailer!.
+        unfold field_address0.
+        destruct (field_compatible0_dec _ _).
+        admit. admit.
+      }
+      rewrite Zlength_cons in H1.
+      change (a :: al) with ([a] ++ al).
+      rewrite (split2_data_at_Tarray_app 1) by Zlength_solve.
+      assert (Zlength al >= 0) by Zlength_solve.
+      rewrite array_pointers_unfold by lia.
+      simpl iter_sepcon.
+      sep_apply data_at_singleton_array_eq. cancel.
+      rewrite H2.
+      apply IHal.
+      lia.
+  - admit.
+Admitted.
+
+Lemma data_at_2darray_concat : forall sh t n m (al : list (list (reptype t))) p,
+  0 <= n ->
+  0 <= m ->
+  Zlength al = n ->
+  Forall (fun l => Zlength l = m) al ->
+  complete_legal_cosu_type t = true ->
+  data_at sh (tarray (tarray t m) n) al p
+    = data_at sh (tarray t (n * m)) (concat al) p.
+Proof.
+  intros.
+  change (list (list (reptype t))) with (list (reptype (tarray t m))) in al.
+  apply pred_ext.
+  - generalize dependent n; generalize dependent p; induction al; intros.
+    + entailer!. rewrite Zlength_nil.
+      sep_apply data_at_zero_array_inv.
+      simpl. replace (0 * m) with 0 by lia.
+      rewrite data_at_zero_array_eq; auto.
+    + assert_PROP (field_address0 (tarray (tarray t m) n) [ArraySubsc 1] p
+          = offset_val (sizeof (tarray t m)) p).
+      {
+        entailer!.
+        unfold field_address0.
+        destruct (field_compatible0_dec _ _).
+        admit.
+        admit.
+      }
+      rewrite Zlength_cons in H1.
+      change (a :: al) with ([a] ++ al).
+      rewrite (split2_data_at_Tarray_app 1) by Zlength_solve.
+
+      simpl concat.
+      change (reptype (tarray t m)) with (list (reptype t)) in a, al.
+      rewrite (split2_data_at_Tarray_app m) by admit.
+Admitted.
+
 Lemma body_main: semax_body Vprog Gprog f_main main_spec.
 Proof.
   start_function.
